imp_system/imp/Imp.v
@@ -177,14 +177,14 @@ Section FB_HAS_SPEC.
       (SPEC : fn_has_spec stb fn fsp)
   .
 
-  Lemma fb_has_spec_weaker (stb : string -> option fspec) (fb : mblock) (fsp0 fsp1 : fspec)
+  Lemma fb_has_weaker_spec (stb : string -> option fspec) (fb : mblock) (fsp0 fsp1 : fspec)
         (SPEC : fb_has_spec stb fb fsp1)
-        (WEAK : fspec_weaker fsp0 fsp1)
+        (WEAK : fspec_imply fsp1 fsp0)
     :
       fb_has_spec stb fb fsp0.
   Proof.
     inv SPEC. econs; eauto.
-    eapply fn_has_spec_weaker; eauto.
+    eapply fn_has_weaker_spec; eauto.
   Qed.
   
 End FB_HAS_SPEC.
@@ -539,20 +539,41 @@ Section MODSEM.
   (* Instance Initial_void1 : @Initial (Type -> Type) IFun void1 := @elim_void1. (*** TODO : move to ITreelib ***) *)
 
   Context `{Σ: GRA}.
-
-  Definition to_itree (ge : GEnv.t) : (string*_) -> (string * (_ * list string * (Any.t -> itree hmodE Any.t)))%type :=
-    (fun '(fn, f) => (fn, (wmask_all, [], cfunU (eval_imp ge f)))).
   
-  Program Definition get_mod (m : program) (ge : GEnv.t) : PMod.t :=
-    {|PMod.scopes := [];
-      PMod.fnsems := List.map (to_itree ge) m.(prog_funs);
-      PMod.initial_st := [];
+  (* TODO : move lemmas to AList.v *)
+  Lemma alist_find_omap_some K `{Dec K} V0 V1 (f : V0 -> V1) (k : K) (l : alist K V0)
+    :
+      alist_find (Some k) (List.map (fun '(k, v) => (Some k, f v)) l) = o_map (alist_find k l) f.
+  Proof using.
+    induction l; ss. uo. destruct a.
+    des_ifs;
+    rewrite eq_rel_dec_correct in Heq1; des_ifs;
+    rewrite eq_rel_dec_correct in Heq; des_ifs.
+  Qed.
+
+  Lemma alist_find_omap_none K `{Dec K} V0 V1 (f : V0 -> V1) (k : K) (l : alist K V0)
+    :
+      alist_find None (List.map (fun '(k, v) => (Some k, f v)) l) = None.
+  Proof using.
+    induction l; ss. uo. destruct a.
+    des_ifs.
+  Qed.
+
+  Definition to_itree (ge : GEnv.t) : (string*_) -> (option string * (fnsem_type (option fspec * fbody)))%type :=
+    (fun '(fn, f) => (Some fn, (false, wmask_all, [], (None, cfunU (eval_imp ge f))))).
+  
+  Program Definition get_mod (m : program) (ge : GEnv.t) : SMod.t :=
+    {|SMod.scopes := [];
+      SMod.fnsems := List.map (to_itree ge) m.(prog_funs);
+      SMod.initial_st := [];
   |}.
   Solve All Obligations with prove_scope.
   Next Obligation.
     ii. unfold HMod.fnsems_scopes, to_itree in *.
-    rewrite ->alist_find_map in *.
-    destruct (alist_find fn (prog_funs m)); ss.
+    destruct fn.
+    - rewrite alist_find_omap_some in H.
+      destruct (alist_find s (prog_funs m)); ss.
+    - rewrite alist_find_omap_none in H; ss.
   Qed.
   Next Obligation. prove_nodup. Qed.
 
