imp_system/imp/ImpProofs.v
@@ -566,7 +566,8 @@ Section PROOFS.
     2:{ rewrite interp_imp_bind. rewrite interp_imp_triggerUB. unfold triggerUB. grind. }
     destruct (is_true v); grind; des_ifs.
     1,2 : rewrite interp_imp_tau; grind.
-    rewrite interp_imp_triggerUB_bind. unfold triggerUB. grind.
+    hexploit (@interp_imp_triggerUB_bind bool val ge l (λ u: bool, tau;; if u then denote_stmt t else denote_stmt e)).
+    rewrite /triggerUB. i; ss. rewrite bind_bind in H. rewrite H. grind.
   Qed.
 
   Lemma interp_imp_AddrOf
@@ -736,9 +737,9 @@ Section PROOFS.
     rewrite interp_imp_bind. rewrite interp_imp_GetName.
     des_ifs.
     1,5,6:(unfold triggerUB; grind).
-    3:{ unfold unwrapU. grind. unfold triggerUB. grind. }
+    3:{ unfold unwrapU. grind. }
     - unfold unwrapU. grind. apply interp_imp_Call_args.
-    - unfold unwrapU. grind. unfold triggerUB; grind.
+    - unfold unwrapU. grind.
   Qed.
 
   Lemma interp_imp_IO_args
@@ -773,7 +774,8 @@ Section PROOFS.
   Proof using.
     rewrite interp_imp_bind. grind.
     des_ifs.
-    2:{ grind. rewrite interp_imp_triggerUB_bind. unfold triggerUB; grind. }
+    2:{ grind. hexploit (@interp_imp_triggerUB_bind unit val ge l (λ u, v <- trigger (IO f (map (λ v, match v with | Vint z => z | _ => 0%Z end) l0));; trigger (SetVar x (Vint v));;; (tau;; Ret Vundef))).
+        rewrite /triggerUB. i; ss. rewrite bind_bind in H. rewrite H. grind. }
     2:{ rewrite interp_imp_bind. rewrite interp_imp_triggerUB. unfold triggerUB; grind. }
     2:{ rewrite interp_imp_triggerUB_bind. unfold triggerUB; grind. }
     rewrite interp_imp_bind. rewrite interp_imp_Ret; grind.
